More tweaks

Wavelet/Determinancy.lean
@@ -9,29 +9,101 @@ namespace Wavelet.Semantics
 
 open Semantics
 
-/-- Restricts an LTS by imposing a state invariant,
-and also transforms the label. -/
-inductive Lts.Guard {S} (InvS : S → Prop) (InvE : E → E' → Prop) (lts : Lts S E) : Lts S E' where
-  | step :
-    InvS s → InvE e e' → InvS s' →
-    lts.Step s e s' →
-    Guard InvS InvE lts s e' s'
+/-- Restricts an LTS by imposing a state invariant. -/
+inductive Lts.Guard {S} (Inv : S → Prop) (lts : Lts S E) : Lts S E where
+  | step : Inv s → Inv s' → lts.Step s e s' → Guard Inv lts s e s'
 
-/-- Guard the transition of a semantics with the given invariant. -/
+/-- Guards the transition of a semantics with the given invariant. -/
 def guard
-  [Arity Op] [Arity Op']
+  [Arity Op]
   (sem : Semantics Op V m n)
-  (InvS : sem.S → Prop)
-  (InvE : Label Op V m n → Label Op' V' m' n' → Prop) :
-  Semantics Op' V' m' n' :=
+  (Inv : sem.S → Prop) :
+  Semantics Op V m n :=
   {
     S := sem.S,
     init := sem.init,
-    lts := sem.lts.Guard InvS InvE,
+    lts := sem.lts.Guard Inv,
     -- TODO: this is actually not true,
     -- maybe remove this requirement?
     yields_functional := sorry
   }
+
+/-- Modifies labels with a relation. -/
+inductive Lts.InterpLabel {S} (Interp : E → E' → Prop) (lts : Lts S E) : Lts S E' where
+  | step : Interp e e' → lts.Step s e s' → InterpLabel Interp lts s e' s'
+
+/-- Interprets the labels as another set of operators. -/
+def interpLabel
+  [Arity Op] [Arity Op']
+  (sem : Semantics Op V m n)
+  (Interp : Label Op V m n → Label Op' V' m' n' → Prop) :
+  Semantics Op' V' m' n' :=
+  {
+    S := sem.S,
+    init := sem.init,
+    lts := sem.lts.InterpLabel Interp,
+    yields_functional := sorry
+  }
+
+/-- Some well-formedness constraints on label interpretations. -/
+class LawfulLabelInterp [Arity Op] [Arity Op']
+  (Interp : Label Op V m n → Label Op' V' m' n' → Prop) where
+  label_interp_tau : Interp .τ .τ
+  label_interp_tau_only : ∀ {l}, Interp .τ l → l.isSilent
+  label_interp_input : ∀ {vals l}, Interp (.input vals) l → l.isSilent ∨ l.isInput
+  label_interp_output : ∀ {vals l}, Interp (.output vals) l → l.isSilent ∨ l.isOutput
+  label_interp_yield : ∀ {op inputs outputs l}, Interp (.yield op inputs outputs) l → l.isSilent ∨ l.isYield
+
+/-- `interpLabel` preserves IO-restricted simulation. -/
+theorem sim_interp_label
+  [Arity Op] [Arity Op']
+  [DecidableEq χ]
+  [DecidableEq χ']
+  [InterpConsts V]
+  [InterpConsts V']
+  {sem₁ sem₂ : Semantics Op V m n}
+  {Interp : Label Op V m n → Label Op' V' m' n' → Prop}
+  [hinterp : LawfulLabelInterp Interp]
+  (hsim : sem₁ ≲ᵣ sem₂) :
+  sem₁.interpLabel Interp ≲ᵣ sem₂.interpLabel Interp
+  := by
+  apply Lts.Similarity.intro hsim.Sim
+  constructor
+  · exact hsim.sim_init
+  · intros s₁ s₂ l s₁' hR hstep
+    simp [Semantics.interpLabel] at hstep
+    cases hstep with | step hlabel hstep =>
+    rename Label Op V m n => l'
+    have ⟨s₂', hstep_s₂, hR₂⟩ := hsim.sim_step _ _ _ _ hR hstep
+    exists s₂'
+    constructor
+    · cases hstep_s₂ with
+      | step_yield hstep_yield_s₂ =>
+        replace hstep_yield_s₂ := Lts.InterpLabel.step hlabel hstep_yield_s₂
+        cases hinterp.label_interp_yield hlabel <;>
+          rename_i h₁ <;> cases l <;> simp at h₁
+        · exact .step_tau (.single hstep_yield_s₂)
+        · exact .step_yield hstep_yield_s₂
+      | step_input hstep_input_s₂ hstep_tau =>
+        replace hstep_input_s₂ := Lts.InterpLabel.step hlabel hstep_input_s₂
+        replace hstep_tau := hstep_tau.map (Lts.InterpLabel.step hinterp.label_interp_tau)
+        cases hinterp.label_interp_input hlabel <;>
+          rename_i h₁ <;> cases l <;> simp at h₁
+        · exact .step_tau (hstep_tau.prepend hstep_input_s₂)
+        · exact .step_input hstep_input_s₂ hstep_tau
+      | step_output hstep_tau hstep_output_s₂ =>
+        replace hstep_output_s₂ := Lts.InterpLabel.step hlabel hstep_output_s₂
+        replace hstep_tau := hstep_tau.map (Lts.InterpLabel.step hinterp.label_interp_tau)
+        cases hinterp.label_interp_output hlabel <;>
+          rename_i h₁ <;> cases l <;> simp at h₁
+        · exact .step_tau (hstep_tau.tail hstep_output_s₂)
+        · exact .step_output hstep_tau hstep_output_s₂
+      | step_tau hstep_tau_s₂ =>
+        replace hstep_tau_s₂ := hstep_tau_s₂.map (Lts.InterpLabel.step hinterp.label_interp_tau)
+        have := hinterp.label_interp_tau_only hlabel
+        cases l <;> simp at this
+        exact .step_tau hstep_tau_s₂
+    · exact hR₂
 
 /-- PCM specification of an operator set -/
 structure OpSpec Op V T [Arity Op] [PCM T] where
@@ -51,8 +123,7 @@ structure IOSpec V T [PCM T] m n where
 to pass a PCM token, as well as two operators to split and join PCMs. -/
 inductive WithSpec (Op : Type u) [Arity Op] [PCM T] (spec : OpSpec Op V T) where
   | op (op : Op)
-  | split
-  | join
+  | join (k : Nat) -- Number of input tokens to combine
 
 /-- Uses only the LHS `InterpConsts` of a sum for constants. -/
 instance instInterpConstsSum [left : InterpConsts V] : InterpConsts (V ⊕ V') where
@@ -74,15 +145,13 @@ instance instArityWithSpec
   {spec : OpSpec Op V T} :
   Arity (WithSpec Op spec) where
   ι | .op o => arity.ι o + 1
-    | .split => 1
-    | .join => 2
+    | .join k => k
   ω | .op o => arity.ω o + 1
-    | .split => 2
-    | .join => 1
+    | .join _ => 2
 
 /-- Interprets the labels with ghost values using the base operators,
 but with dynamic checks for ghost tokens satisfying the specs. -/
-inductive SpecLabelInv [Arity Op] [PCM T]
+inductive SpecLabelInterp [Arity Op] [PCM T]
   (opSpec : OpSpec Op V T)
   (ioSpec : IOSpec V T m n) :
   Label (WithSpec Op opSpec) (V ⊕ T) (m + 1) (n + 1) → Label Op V m n → Prop where
@@ -93,43 +162,47 @@ inductive SpecLabelInv [Arity Op] [PCM T]
     outputs'.back = .inr tok₂ →
     tok₁ ≡ opSpec.pre op inputs →
     tok₂ ≡ opSpec.post op inputs outputs →
-    SpecLabelInv opSpec ioSpec
+    SpecLabelInterp opSpec ioSpec
       (.yield (.op op) inputs' outputs')
       (.yield op inputs outputs)
-  -- NOTE: the exact split of permissions is
-  -- intentionally left unspecified, because
+  -- NOTE: the exact output split of permissions
+  -- is intentionally left unspecified, because
   -- we want this to be dynamic without restricting
   -- to a static annotation.
-  | spec_split
-    {inputs : Vector (V ⊕ T) 1}
-    {outputs : Vector (V ⊕ T) 2} :
-    inputs[0] = .inr tok₁ →
-    outputs[0] = .inr tok₂ →
-    outputs[1] = .inr tok₃ →
-    tok₁ ≡ tok₂ ⊔ tok₃ →
-    SpecLabelInv opSpec ioSpec
-      (.yield .split inputs outputs) .τ
   | spec_join
-    {inputs : Vector (V ⊕ T) 2}
-    {outputs : Vector (V ⊕ T) 1} :
-    inputs[0] = .inr tok₁ →
-    inputs[1] = .inr tok₂ →
-    outputs[0] = .inr tok₃ →
-    tok₃ ≡ tok₁ ⊔ tok₂ →
-    SpecLabelInv opSpec ioSpec
-      (.yield .join inputs outputs) .τ
+    {inputs : Vector (V ⊕ T) k}
+    {toks : Vector T k}
+    {outputs : Vector (V ⊕ T) 2} :
+    inputs = toks.map .inr →
+    outputs[0] = .inr tok₁ →
+    outputs[1] = .inr tok₂ →
+    tok₁ ⊔ tok₂ ≡ PCM.sum toks.toList →
+    SpecLabelInterp opSpec ioSpec
+      (.yield (.join k) inputs outputs) .τ
   | spec_input :
     vals'.pop = vals.map .inl →
     vals'.back = .inr tok →
     tok ≡ ioSpec.pre vals →
-    SpecLabelInv opSpec ioSpec
+    SpecLabelInterp opSpec ioSpec
       (.input vals') (.input vals)
   | spec_output :
     vals'.pop = vals.map .inl →
     vals'.back = .inr tok →
     tok ≡ ioSpec.post vals →
-    SpecLabelInv opSpec ioSpec
+    SpecLabelInterp opSpec ioSpec
       (.output vals') (.output vals)
+  | spec_tau :
+    SpecLabelInterp opSpec ioSpec .τ .τ
+
+instance
+  [Arity Op] [PCM T]
+  {opSpec : OpSpec Op V T}
+  {ioSpec : IOSpec V T m n} : LawfulLabelInterp (SpecLabelInterp opSpec ioSpec) where
+  label_interp_tau := .spec_tau
+  label_interp_tau_only h := by cases h; rfl
+  label_interp_input h := by cases h; simp
+  label_interp_output h := by cases h; simp
+  label_interp_yield h := by cases h <;> simp
 
 end Wavelet.Semantics
 
@@ -146,10 +219,16 @@ def Config.DisjointTokens
     c.vars.getVar x₂ = some (.inr t₂) →
     t₁ ⊥ t₂
 
-abbrev FnWithSpec
+abbrev ExprWithSpec
   [Arity Op] [PCM T]
   (opSpec : Semantics.OpSpec Op V T)
   (_ioSpec : IOSpec V T m n) χ m n
+  := Expr (WithSpec Op opSpec) χ (m + 1) (n + 1)
+
+abbrev FnWithSpec
+  [Arity Op] [PCM T]
+  (opSpec : Semantics.OpSpec Op V T)
+  (_ioSpec : IOSpec V T m n) χ
   := Fn (WithSpec Op opSpec) χ (V ⊕ T) (m + 1) (n + 1)
 
 end Wavelet.Seq
@@ -225,68 +304,10 @@ theorem sim_compile_fn'
   [DecidableEq χ]
   {opSpec : Semantics.OpSpec Op V T}
   {ioSpec : IOSpec V T m n}
-  (fn : FnWithSpec opSpec ioSpec χ m n)
+  (fn : FnWithSpec opSpec ioSpec χ)
   (hwf : fn.AffineVar) :
-  fn.semantics.guard Config.DisjointTokens (SpecLabelInv opSpec ioSpec)
-    ≲ᵣ (compileFn (by simp) fn).semantics.guard Config.DisjointTokens (SpecLabelInv opSpec ioSpec)
-  := sorry
-
-theorem sim_guard_label
-  [Arity Op] [Arity Op']
-  [DecidableEq χ]
-  [DecidableEq χ']
-  [InterpConsts V]
-  [InterpConsts V']
-  {sem₁ sem₂ : Semantics Op V m n}
-  {InvE : Label Op V m n → Label Op' V' m' n' → Prop}
-  (htau : InvE .τ .τ)
-  (hinput : ∀ {vals l}, InvE (.input vals) l → l.isSilent ∨ l.isInput)
-  (houtput : ∀ {vals l}, InvE (.output vals) l → l.isSilent ∨ l.isOutput)
-  (hyield : ∀ {op inputs outputs l}, InvE (.yield op inputs outputs) l → l.isSilent ∨ l.isYield)
-  (hsim : sem₁ ≲ᵣ sem₂) :
-  sem₁.guard (λ _ => True) InvE ≲ᵣ sem₂.guard (λ _ => True) InvE
-  := by
-  apply Lts.Similarity.intro hsim.Sim
-  constructor
-  · exact hsim.sim_init
-  · intros s₁ s₂ l s₁' hR hstep
-    simp [Semantics.guard] at hstep
-    cases hstep with | step _ hlabel _ hstep =>
-    rename Label Op V m n => l'
-    have ⟨s₂', hstep_s₂, hR₂⟩ := hsim.sim_step _ _ _ _ hR hstep
-    exists s₂'
-    constructor
-    · cases l' with
-      | yield => sorry
-      | input =>
-        cases hstep_s₂ with | step_input hstep_input_s₂ hstep_tau =>
-        sorry
-      | output => sorry
-      | τ => sorry
-    · exact hR₂
-
-/-- Type check a function against the given specs,
-and insert split/join to concretize the flow of permissions. -/
-def typeCheck
-  [Arity Op]
-  [PCM T]
-  (opSpec : Semantics.OpSpec Op V T)
-  (ioSpec : IOSpec V T m n)
-  (fn : Fn Op χ V m n) : Option (FnWithSpec opSpec ioSpec χ m n) := sorry
-
-/-- Type soundness theorem formulated as a simulation. -/
-theorem fn_progress
-  [Arity Op]
-  [InterpConsts V]
-  [PCM T]
-  [DecidableEq χ]
-  {opSpec : Semantics.OpSpec Op V T}
-  {ioSpec : IOSpec V T m n}
-  (fn : Fn Op χ V m n)
-  {fn' : FnWithSpec opSpec ioSpec χ m n}
-  (hwf : fn.AffineVar)
-  (hwt : typeCheck opSpec ioSpec fn = some fn') :
-  fn.semantics ≲ᵣ fn'.semantics.guard Config.DisjointTokens (SpecLabelInv opSpec ioSpec)
+  fn.semantics.guard Config.DisjointTokens
+    ≲ᵣ (compileFn (by simp) fn).semantics.guard Config.DisjointTokens
   := sorry
 
 /-- Erase ghost tokens. -/
@@ -307,7 +328,7 @@ theorem sim_erase_ghost
   {ioSpec : IOSpec V T m n}
   (proc : ProcWithSpec opSpec ioSpec χ m n) :
   (eraseGhost proc).semantics ≲ᵣ
-    proc.semantics.guard Config.DisjointTokens (SpecLabelInv opSpec ioSpec)
+    (proc.semantics.guard Config.DisjointTokens).interpLabel (SpecLabelInterp opSpec ioSpec)
   := sorry
 
 /-- Forward simulation for liveness. -/
@@ -319,7 +340,7 @@ theorem sim_erase_ghost_forward
   {opSpec : Semantics.OpSpec Op V T}
   {ioSpec : IOSpec V T m n}
   (proc : ProcWithSpec opSpec ioSpec χ m n) :
-  proc.semantics.guard Config.DisjointTokens (SpecLabelInv opSpec ioSpec)
+  (proc.semantics.guard Config.DisjointTokens).interpLabel (SpecLabelInterp opSpec ioSpec)
     ≲ᵣ (eraseGhost proc).semantics
   := sorry
 
@@ -337,7 +358,7 @@ theorem guarded_confluence
   {trace₁ trace₂ : Trace (Label Op V m n)}
   {sem : Semantics Op V m n}
   {s₁ s₂ : sem.S}
-  {hguard : sem = proc.semantics.guard Config.DisjointTokens (SpecLabelInv opSpec ioSpec)}
+  {hguard : sem = (proc.semantics.guard Config.DisjointTokens).interpLabel (SpecLabelInterp opSpec ioSpec)}
   (htrace₁ : sem.lts.Star sem.init trace₁ s₁)
   (htrace₂ : sem.lts.Star sem.init trace₂ s₂) :
   ∃ trace₁' trace₂' s₁' s₂',
@@ -348,3 +369,127 @@ theorem guarded_confluence
   := sorry
 
 end Wavelet.Compile
+
+namespace Wavelet.Seq
+
+open Semantics
+
+/-- Simple non-dependent resource specs. -/
+structure SimpleOpSpec Op T [PCM T] where
+  pre : Op → T
+  post : Op → T
+  frame_preserving : ∀ op, pre op ⟹ post op
+
+def SimpleOpSpec.toOpSpec
+  V [Arity Op] [PCM T]
+  (spec : SimpleOpSpec Op T) :
+  Semantics.OpSpec Op V T := {
+    pre op _ := spec.pre op,
+    post op _ _ := spec.post op,
+    frame_preserving := by intros; apply spec.frame_preserving
+  }
+
+structure SimpleIOSpec T [PCM T] where
+  pre : T
+  post : T
+
+def SimpleIOSpec.toIOSpec
+  [PCM T]
+  (spec : SimpleIOSpec T) m n :
+  IOSpec V T m n := {
+    pre _ := spec.pre,
+    post _ := spec.post,
+  }
+
+inductive TypedName χ where
+  | var (x : χ)
+  | tok (i : Nat)
+  deriving DecidableEq
+
+/-- Tries to find a set of `ts : Fin numToks`
+such that `req ≤ sum of (ts.map ctx)`. -/
+def tryAcquire
+  (ctx : Nat → Option T)
+  (numToks : Nat)
+  (req : T) : Option (List Nat) :=
+  sorry
+
+/-- Helper function for `typeCheck`. -/
+noncomputable def typeCheckInternal
+  [Arity Op] [PCM T]
+  [DecidableLE T]
+  (opSpec : SimpleOpSpec Op T)
+  (ioSpec : SimpleIOSpec T)
+  (ctx : Nat → Option T)
+  (numToks : Nat) :
+  Expr Op χ m n →
+  Option (ExprWithSpec (opSpec.toOpSpec V) (ioSpec.toIOSpec m n) (TypedName χ) m n)
+  | .ret args => do
+    let toks ← tryAcquire ctx numToks ioSpec.post
+    return .op (.join toks.length)
+      (toks.toVector.map .tok)
+      #v[.tok numToks, .tok (numToks + 1)]
+      (.ret ((args.map .var).push (.tok numToks)))
+  | .tail args => do
+    let toks ← tryAcquire ctx numToks ioSpec.pre
+    return .op (.join toks.length)
+      (toks.toVector.map .tok)
+      #v[.tok numToks, .tok (numToks + 1)]
+      (.tail ((args.map .var).push (.tok numToks)))
+  | .op o args bind cont => do
+    let toks ← tryAcquire ctx numToks (opSpec.pre o)
+    let tok₁ := .tok numToks
+    let tok₂ := .tok (numToks + 1)
+    let tok₃ := .tok (numToks + 2)
+    let newCtx₁ := λ i => if i ∈ toks then none else ctx i
+    let newCtx₂ := Function.update newCtx₁ numToks (some (opSpec.pre o))
+    let sumToks ← toks.foldlM (λ acc i => return acc ⊔ (← ctx i)) PCM.zero
+    if h : opSpec.pre o ≤ sumToks then
+      let newCtx₃ := Function.update newCtx₂ (numToks + 1) (some (PCM.sub sumToks (opSpec.pre o) h))
+      let newCtx₄ := Function.update newCtx₃ (numToks + 2) (some (opSpec.post o))
+      return .op (.join toks.length) (toks.toVector.map .tok) #v[tok₁, tok₂]
+        (.op (.op o)
+          ((args.map .var).push tok₁)
+          ((bind.map .var).push tok₃)
+          (← typeCheckInternal opSpec ioSpec newCtx₄ (numToks + 3) cont))
+    else
+      none
+  | .br cond left right => do
+    let left' ← typeCheckInternal opSpec ioSpec ctx numToks left
+    let right' ← typeCheckInternal opSpec ioSpec ctx numToks right
+    return .br (.var cond) left' right'
+
+/-- Type check a function against the given specs,
+and insert split/join to concretize the flow of permissions. -/
+noncomputable def typeCheck
+  [Arity Op] [PCM T]
+  [DecidableLE T]
+  (opSpec : SimpleOpSpec Op T)
+  (ioSpec : SimpleIOSpec T)
+  (fn : Fn Op χ V m n) :
+  Option (FnWithSpec (opSpec.toOpSpec V) (ioSpec.toIOSpec m n) (TypedName χ))
+  := return {
+    params := (fn.params.map TypedName.var).push (TypedName.tok 0),
+    body := ← typeCheckInternal opSpec ioSpec
+      (Function.update (Function.const _ none) 0 (some ioSpec.pre)) 1 fn.body,
+  }
+
+/-- Type soundness theorem formulated as a simulation. -/
+theorem type_check_sound
+  [Arity Op]
+  [InterpConsts V]
+  [PCM T]
+  [DecidableEq χ]
+  [DecidableLE T]
+  (opSpec : SimpleOpSpec Op T)
+  (ioSpec : SimpleIOSpec T)
+  (fn : Fn Op χ V m n)
+  {fn' : FnWithSpec (opSpec.toOpSpec V) (ioSpec.toIOSpec m n) (TypedName χ)}
+  (hwf : fn.AffineVar)
+  (hwt : typeCheck opSpec ioSpec fn = some fn') :
+  fn.semantics ≲ᵣ
+    (fn'.semantics.guard Config.DisjointTokens).interpLabel
+      (SpecLabelInterp (opSpec.toOpSpec V) (ioSpec.toIOSpec m n))
+  := sorry
+
+end Wavelet.Seq
